continue porting

concurrency/framework/StateMachines.s.dfy
@@ -81,6 +81,62 @@ module AsyncStateMachine(IOIfc: InputOutputIfc, SM: StateMachine(IOIfc))
   }
 }
 
+// Alternate version, used by the older hash table case study
+module AsyncStateMachineWithMultisets(IOIfc: InputOutputIfc, SM: StateMachine(IOIfc))
+    refines StateMachine(AsyncIfc(IOIfc))
+{
+  import opened RequestIds
+
+  datatype Req = Req(rid: RequestId, input: IOIfc.Input)
+  datatype Resp = Resp(rid: RequestId, output: IOIfc.Output)
+
+  datatype Variables = Variables(
+      s: SM.Variables,
+      reqs: multiset<Req>,
+      resps: multiset<Resp>)
+
+  predicate Init(s: Variables)
+  {
+    && SM.Init(s.s)
+    && s.reqs == multiset{}
+    && s.resps == multiset{}
+  }
+
+  predicate LinearizationPoint(s: Variables, s': Variables,
+      rid: RequestId, input: IOIfc.Input, output: IOIfc.Output)
+  {
+    // resolve request step
+    // serialization point: remove 'input' from 'reqs',
+    // add 'output' to 'resps'
+    && Req(rid, input) in s.reqs
+    && s.reqs == s'.reqs + multiset{Req(rid, input)}
+    && s'.resps == s.resps + multiset{Resp(rid, output)}
+    && SM.Next(s.s, s'.s, IOIfc.Op(input, output))
+  }
+
+  predicate Next(s: Variables, s': Variables, op: ifc.Op)
+  {
+    match op {
+      case Start(rid, input) =>
+        // add 'input' to 'reqs'
+        && s' == s.(reqs := s.reqs + multiset{Req(rid, input)})
+      case InternalOp => (
+        // stutter step
+        || (s' == s)
+
+        // resolve request step
+        || (exists rid, input, output ::
+          LinearizationPoint(s, s', rid, input, output)
+        )
+      )
+      case End(rid, output) =>
+        // remove from 'resps'
+        && Resp(rid, output) in s.resps
+        && s' == s.(resps := s.resps - multiset{Resp(rid, output)})
+    }
+  }
+}
+
 abstract module Refinement(ifc: Ifc, A: StateMachine(ifc), B: StateMachine(ifc)) {
   predicate Inv(s: A.Variables)
 
